Progress on step_delay proof with the new statement

pancake/proofs/ffiTimeScript.sml
@@ -9,46 +9,37 @@ val _ = set_grammar_ancestry
         ["panSem",
          "multiword"];
 
+Type time_input = ``:num -> num # bool``
 
+Type time_input_ffi = ``:time_input ffi_state``
 
-Type time = ``:num -> num``
-
-Type time_ffi = ``:time ffi_state``
-
-Type time_oracle = ``:string -> time oracle_function``
-
-Type pan_state = ``:('a, time) panSem$state``
-
-
-
-Definition time_seq_def:
-  time_seq (f:num -> num) =
-    ∀n. f n ≤ f (SUC n)
-End
-
-
-Definition nffi_def:
-  nffi (f:num -> num) =
-   λn. f (n+1)
-End
+Type pan_state = ``:('a, time_input) panSem$state``
 
 Overload k2mw = “multiword$k2mw”
 
-Definition nffi_def:
-  nbytes (f:num -> num) n =
-    (k2mw n (f 0)):word8 list
+
+Definition next_ffi_def:
+  next_ffi (f:num -> (num # bool)) =
+    λn. f (n+1)
 End
 
-(* n = dimindex (:α) DIV 8 *)
+
+Definition ntime_input_def:
+  ntime_input (f:num -> num # bool) n =
+    ((k2mw (n-1) (FST (f 0))):word8 list) ++
+    [if SND (f 0) then 0w else 1w]
+End
+
+
 Definition build_ffi_def:
-  build_ffi (seq:time) =
+  build_ffi (seq:time_input) =
      <| oracle    :=
         (λs f conf bytes.
-          if s = "get_time"
-          then Oracle_return (nffi f) (nbytes f (LENGTH bytes))
+          if s = "get_ffi"
+          then Oracle_return (next_ffi f) (ntime_input f (LENGTH bytes))
           else Oracle_final FFI_failed)
       ; ffi_state := seq
-      ; io_events := [] |> : time_ffi
+      ; io_events := [] |> : time_input_ffi
 End
 
 
